Map for Ref.
* Also, removed the box from the definition of typing judgments, so that we can frame resources around them.

theories/typing/programs.v
@@ -10,7 +10,7 @@ Section typing.
   (* This is an iProp because it is also used by the function type. *)
   Definition typed_body (E : elctx) (L : llctx) (C : cctx) (T : tctx)
                         (e : expr) : iProp Σ :=
-    (□ ∀ tid qE, lft_ctx -∗ na_own tid ⊤ -∗
+    (∀ tid qE, lft_ctx -∗ na_own tid ⊤ -∗
                elctx_interp E qE -∗ llctx_interp L 1 -∗
                (elctx_interp E qE -∗ cctx_interp tid C) -∗ tctx_interp tid T -∗
                WP e {{ _, cont_postcondition }})%I.
@@ -34,7 +34,7 @@ Section typing.
     Proper (flip (cctx_incl E) ==> flip (tctx_incl E L) ==> eq ==> (⊢))
            (typed_body E L).
   Proof.
-    intros C1 C2 HC T1 T2 HT e ? <-. iIntros "#H !#".
+    intros C1 C2 HC T1 T2 HT e ? <-. iIntros "H".
     iIntros (tid qE) "#LFT Htl HE HL HC HT".
     iMod (HT with "LFT HE HL HT") as "(HE & HL & HT)".
     iApply ("H" with "LFT Htl HE HL [HC] HT").
@@ -49,7 +49,7 @@ Section typing.
   (** Instruction *)
   Definition typed_instruction (E : elctx) (L : llctx)
              (T1 : tctx) (e : expr) (T2 : val → tctx) : iProp Σ :=
-    (□ ∀ tid qE, lft_ctx -∗ na_own tid ⊤ -∗
+    (∀ tid qE, lft_ctx -∗ na_own tid ⊤ -∗
               elctx_interp E qE -∗ llctx_interp L 1 -∗ tctx_interp tid T1 -∗
               WP e {{ v, na_own tid ⊤ ∗ elctx_interp E qE ∗
                          llctx_interp L 1 ∗ tctx_interp tid (T2 v) }})%I.
@@ -98,7 +98,7 @@ Section typing_rules.
     typed_body ((κ1 ⊑ κ2) :: (κ2 ⊑ κ1) :: E) L C T e →
     typed_body E ((κ1 ⊑ [κ2]%list) :: L) C T e.
   Proof.
-    iIntros (He) "!#". iIntros (tid qE) "#LFT Htl HE HL HC HT".
+    iIntros (He tid qE) "#LFT Htl HE HL HC HT".
     rewrite /llctx_interp big_sepL_cons. iDestruct "HL" as "[Hκ HL]".
     iMod (lctx_equalize_lft with "LFT Hκ") as "[Hκ1 Hκ2]".
     iApply (He with "LFT Htl [Hκ1 Hκ2 HE] HL [HC] HT").
@@ -113,8 +113,8 @@ Section typing_rules.
     (∀ v : val, typed_body E L C (T2 v ++ T) (subst' xb v e')) -∗
     typed_body E L C (T1 ++ T) (let: xb := e in e').
   Proof.
-    iIntros (Hc) "#He #He' !#". iIntros (tid qE) "#LFT Htl HE HL HC HT". rewrite tctx_interp_app.
-    iDestruct "HT" as "[HT1 HT]". wp_bind e. iApply (wp_wand with "[HE HL HT1 Htl]").
+    iIntros (Hc) "He He'". iIntros (tid qE) "#LFT Htl HE HL HC HT". rewrite tctx_interp_app.
+    iDestruct "HT" as "[HT1 HT]". wp_bind e. iApply (wp_wand with "[He HE HL HT1 Htl]").
     { iApply ("He" with "LFT Htl HE HL HT1"). }
     iIntros (v) "/= (Htl & HE & HL & HT2)". iApply wp_let; first wp_done.
     iModIntro. iApply ("He'" with "LFT Htl HE HL HC [HT2 HT]").
@@ -150,7 +150,7 @@ Section typing_rules.
     (∀ κ, typed_body E ((κ ⊑ κs) :: L) C T e) -∗
     typed_body E L C T (Newlft ;; e).
   Proof.
-    iIntros (Hc) "#He !#". iIntros (tid qE) "#LFT Htl HE HL HC HT".
+    iIntros (Hc) "He". iIntros (tid qE) "#LFT Htl HE HL HC HT".
     iMod (lft_create with "LFT") as (Λ) "[Htk #Hinh]"; first done.
     set (κ' := foldr (∪) static κs). wp_seq.
     iApply ("He" $! (κ' ∪ Λ) with "LFT Htl HE [HL Htk] HC HT").
@@ -164,7 +164,7 @@ Section typing_rules.
     Closed [] e → UnblockTctx κ T1 T2 →
     typed_body E L C T2 e -∗ typed_body E ((κ ⊑ κs) :: L) C T1 (Endlft ;; e).
   Proof.
-    iIntros (Hc Hub) "#He !#". iIntros (tid qE) "#LFT Htl HE".
+    iIntros (Hc Hub) "He". iIntros (tid qE) "#LFT Htl HE".
     rewrite /llctx_interp big_sepL_cons. iIntros "[Hκ HL] HC HT".
     iDestruct "Hκ" as (Λ) "(% & Htok & #Hend)".
     iSpecialize ("Hend" with "Htok"). wp_bind Endlft.
@@ -176,7 +176,7 @@ Section typing_rules.
   Lemma type_path_instr {E L} p ty :
     typed_instruction_ty E L [p ◁ ty] p ty.
   Proof.
-    iIntros "!# * _ $$$ ?". rewrite tctx_interp_singleton.
+    iIntros (??) "_ $$$ ?". rewrite tctx_interp_singleton.
     iApply (wp_hasty with "[-]"). done. iIntros (v) "_ Hv".
     rewrite tctx_interp_singleton. iExists v. iFrame. by rewrite eval_path_of_val.
   Qed.
@@ -192,7 +192,7 @@ Section typing_rules.
     typed_write E L ty1 ty ty1' →
     typed_instruction E L [p1 ◁ ty1; p2 ◁ ty] (p1 <- p2) (λ _, [p1 ◁ ty1']%TC).
   Proof.
-    iIntros (Hwrt) "!#". iIntros (tid qE) "#LFT $ HE HL".
+    iIntros (Hwrt tid qE) "#LFT $ HE HL".
     rewrite tctx_interp_cons tctx_interp_singleton. iIntros "[Hp1 Hp2]".
     wp_bind p1. iApply (wp_hasty with "Hp1"). iIntros (v1) "% Hown1".
     wp_bind p2. iApply (wp_hasty with "Hp2"). iIntros (v2) "_ Hown2".
@@ -218,7 +218,7 @@ Section typing_rules.
     ty.(ty_size) = 1%nat → typed_read E L ty1 ty ty1' →
     typed_instruction E L [p ◁ ty1] (!p) (λ v, [p ◁ ty1'; v ◁ ty]%TC).
   Proof.
-    iIntros (Hsz Hread) "!#". iIntros (tid qE) "#LFT Htl HE HL Hp".
+    iIntros (Hsz Hread tid qE) "#LFT Htl HE HL Hp".
     rewrite tctx_interp_singleton. wp_bind p. iApply (wp_hasty with "Hp").
     iIntros (v) "% Hown".
     iMod (Hread with "[] LFT Htl HE HL Hown") as
@@ -271,7 +271,7 @@ Section typing_rules.
     typed_instruction E L [p1 ◁ ty1; p2 ◁ ty2] (p1 <-{n} !p2)
                       (λ _, [p1 ◁ ty1'; p2 ◁ ty2']%TC).
   Proof.
-    iIntros (Hsz Hwrt Hread) "!#". iIntros (tid qE) "#LFT Htl HE HL HT".
+    iIntros (Hsz Hwrt Hread tid qE) "#LFT Htl HE HL HT".
     iApply (type_memcpy_iris with "[] [] [$LFT $Htl $HE $HL HT]"); try done.
     { iApply Hwrt. }
     { iApply Hread. }
