theories/typing/bool.v
@@ -26,7 +26,7 @@ Section typing.
   Lemma type_bool_instr (b : Datatypes.bool) E L :
     typed_instruction_ty E L [] #b bool.
   Proof.
-    iAlways. iIntros (tid qE) "_ $ $ $ _". wp_value.
+    iIntros (tid qE) "_ $ $ $ _". wp_value.
     rewrite tctx_interp_singleton tctx_hasty_val. by destruct b.
   Qed.
 
@@ -41,7 +41,7 @@ Section typing.
     typed_body E L C T e1 -∗ typed_body E L C T e2 -∗
     typed_body E L C T (if: p then e1 else e2).
   Proof.
-    iIntros (Hp) "#He1 #He2 !#". iIntros (tid qE) "#LFT Htl HE HL HC HT".
+    iIntros (Hp) "He1 He2". iIntros (tid qE) "#LFT Htl HE HL HC HT".
     iDestruct (big_sepL_elem_of _ _ _ Hp with "HT") as "#Hp".
     wp_bind p. iApply (wp_hasty with "Hp").
     iIntros ([[| |[|[]|]]|]) "_ H1"; try done; (iApply wp_case; [done..|iNext]).
