theories/typing/borrow.v
@@ -47,7 +47,7 @@ Section borrow.
     lctx_lft_alive E L κ →
     typed_instruction_ty E L [p ◁ &uniq{κ} own_ptr n ty] (!p) (&uniq{κ} ty).
   Proof.
-    iIntros (Hκ) "!#". iIntros (tid qE) "#LFT $ HE HL Hp".
+    iIntros (Hκ tid qE) "#LFT $ HE HL Hp".
     rewrite tctx_interp_singleton.
     iMod (Hκ with "HE HL") as (q) "[Htok Hclose]"; first set_solver.
     wp_apply (wp_hasty with "Hp"). iIntros ([[]|]) "_ Hown"; try done.
@@ -77,7 +77,7 @@ Section borrow.
     lctx_lft_alive E L κ →
     typed_instruction_ty E L [p ◁ &shr{κ} own_ptr n ty] (!p) (&shr{κ} ty).
   Proof.
-    iIntros (Hκ) "!#". iIntros (tid qE) "#LFT $ HE HL Hp".
+    iIntros (Hκ tid qE) "#LFT $ HE HL Hp".
     rewrite tctx_interp_singleton.
     iMod (Hκ with "HE HL") as (q) "[[Htok1 Htok2] Hclose]"; first set_solver.
     wp_apply (wp_hasty with "Hp"). iIntros ([[]|]) "_ Hown"; try done.
@@ -103,7 +103,7 @@ Section borrow.
     lctx_lft_alive E L κ → lctx_lft_incl E L κ κ' →
     typed_instruction_ty E L [p ◁ &uniq{κ} &uniq{κ'} ty] (!p) (&uniq{κ} ty).
   Proof.
-    iIntros (Hκ Hincl) "!#". iIntros (tid qE) "#LFT $ HE HL Hp".
+    iIntros (Hκ Hincl tid qE) "#LFT $ HE HL Hp".
     rewrite tctx_interp_singleton.
     iPoseProof (Hincl with "[#] [#]") as "Hincl".
     { by iApply elctx_interp_persist. } { by iApply llctx_interp_persist. }
@@ -137,7 +137,7 @@ Section borrow.
     lctx_lft_alive E L κ → lctx_lft_incl E L κ κ' →
     typed_instruction_ty E L [p ◁ &shr{κ} &uniq{κ'} ty] (!p) (&shr{κ} ty).
   Proof.
-    iIntros (Hκ Hincl) "!# * #LFT $ HE HL Hp". rewrite tctx_interp_singleton.
+    iIntros (Hκ Hincl tid qE) "#LFT $ HE HL Hp". rewrite tctx_interp_singleton.
     iPoseProof (Hincl with "[#] [#]") as "Hincl".
     { by iApply elctx_interp_persist. } { by iApply llctx_interp_persist. }
     iMod (Hκ with "HE HL") as (q) "[[Htok1 Htok2] Hclose]"; first set_solver.
