theories/typing/cont.v
@@ -13,7 +13,7 @@ Section typing.
     tctx_incl E L T (T' (list_to_vec args)) →
     typed_body E L C T (k (of_val <$> args)).
   Proof.
-    iIntros (HC Hincl) "!#". iIntros (tid qE) "#LFT Htl HE HL HC HT".
+    iIntros (HC Hincl tid qE) "#LFT Htl HE HL HC HT".
     iMod (Hincl with "LFT HE HL HT") as "(HE & HL & HT)".
     iSpecialize ("HC" with "HE []"); first done.
     rewrite -{3}(vec_to_list_of_list args). iApply ("HC" with "Htl HL HT").
@@ -22,18 +22,37 @@ Section typing.
   Lemma type_cont argsb L1 (T' : vec val (length argsb) → _) E L2 C T econt e2 kb :
     Closed (kb :b: argsb +b+ []) econt → Closed (kb :b: []) e2 →
     (∀ k, typed_body E L2 (k ◁cont(L1, T') :: C) T (subst' kb k e2)) -∗
-    (∀ k (args : vec val (length argsb)),
-       typed_body E L1 (k ◁cont(L1, T') :: C) (T' args) (subst_v (kb::argsb) (k:::args) econt)) -∗
+    □ (∀ k (args : vec val (length argsb)),
+          typed_body E L1 (k ◁cont(L1, T') :: C) (T' args)
+                     (subst_v (kb::argsb) (k:::args) econt)) -∗
     typed_body E L2 C T (e2 cont: kb argsb := econt).
   Proof.
-    iIntros (Hc1 Hc2) "#He2 #Hecont !#". iIntros (tid qE) "#LFT Htl HE HL HC HT". iApply wp_let'.
-    { simpl. rewrite decide_left. done. }
-    iModIntro. iApply ("He2" with "LFT Htl HE HL [HC] HT"). iClear "He2".
+    iIntros (Hc1 Hc2) "He2 #Hecont". iIntros (tid qE) "#LFT Htl HE HL HC HT".
+    iApply wp_let'; first by rewrite /= decide_left.
+    iModIntro. iApply ("He2" with "LFT Htl HE HL [HC] HT").
     iIntros "HE". iLöb as "IH". iIntros (x) "H".
     iDestruct "H" as %[->|?]%elem_of_cons; last by iApply ("HC" with "HE").
     iIntros (args) "Htl HL HT". iApply wp_rec; try done.
     { rewrite Forall_fmap Forall_forall=>? _. rewrite /= to_of_val. eauto. }
     { by rewrite -(subst_v_eq (_ :: _) (RecV _ _ _ ::: _)). }
     iNext. iApply ("Hecont" with "LFT Htl HE HL [HC] HT"). by iApply "IH".
+  Qed.
+
+  Lemma type_cont_norec argsb L1 (T' : vec val (length argsb) → _) E L2 C T econt e2 kb :
+    Closed (kb :b: argsb +b+ []) econt → Closed (kb :b: []) e2 →
+    (∀ k, typed_body E L2 (k ◁cont(L1, T') :: C) T (subst' kb k e2)) -∗
+    (∀ k (args : vec val (length argsb)),
+          typed_body E L1 C (T' args) (subst_v (kb :: argsb) (k:::args) econt)) -∗
+    typed_body E L2 C T (e2 cont: kb argsb := econt).
+  Proof.
+    iIntros (Hc1 Hc2) "He2 Hecont". iIntros (tid qE) "#LFT Htl HE HL HC HT".
+    iApply wp_let'; first by rewrite /= decide_left.
+    iModIntro. iApply ("He2" with "LFT Htl HE HL [HC Hecont] HT").
+    iIntros "HE". iIntros (x) "H".
+    iDestruct "H" as %[->|?]%elem_of_cons; last by iApply ("HC" with "HE").
+    iIntros (args) "Htl HL HT". iApply wp_rec; try done.
+    { rewrite Forall_fmap Forall_forall=>? _. rewrite /= to_of_val. eauto. }
+    { by rewrite -(subst_v_eq (_ :: _) (RecV _ _ _ ::: _)). }
+    iNext. iApply ("Hecont" with "LFT Htl HE HL HC HT").
   Qed.
 End typing.
