theories/typing/examples/init_prod.v
@@ -16,7 +16,8 @@ Section init_prod.
     typed_instruction_ty [] [] [] init_prod
         (fn([]; int, int) → Π[int;int]).
   Proof.
-    iApply type_fn; [solve_typing..|]. simpl. iIntros ([] ret p). inv_vec p=>x y. simpl_subst.
+    iApply type_fn; [solve_typing..|]. iIntros "/= !#". iIntros ([] ret p).
+      inv_vec p=>x y. simpl_subst.
     iApply type_deref; [solve_typing..|apply read_own_move|done|]. iIntros (x'). simpl_subst.
     iApply type_deref; [solve_typing..|apply read_own_move|done|]. iIntros (y'). simpl_subst.
     iApply (type_new_subtype (Π[uninit 1; uninit 1])); [solve_typing..|].
