theories/typing/examples/option_as_mut.v
@@ -19,10 +19,12 @@ Section option_as_mut.
     typed_instruction_ty [] [] [] option_as_mut
         (fn(∀ α, [☀α]; &uniq{α} Σ[unit; τ]) → Σ[unit; &uniq{α}τ]).
   Proof.
-    iApply type_fn; [solve_typing..|]. simpl. iIntros (α ret p). inv_vec p=>o. simpl_subst.
+    iApply type_fn; [solve_typing..|]. iIntros "/= !#". iIntros (α ret p).
+      inv_vec p=>o. simpl_subst.
     iApply (type_cont [_] [] (λ r, [o ◁ _; r!!!0 ◁ _])%TC) ; [solve_typing..| |].
     - iIntros (k). simpl_subst.
-      iApply type_deref; [solve_typing|apply read_own_move|done|]. iIntros (o'). simpl_subst.
+      iApply type_deref; [solve_typing|apply read_own_move|done|].
+        iIntros (o'). simpl_subst.
       iApply type_new; [solve_typing..|]. iIntros (r). simpl_subst.
       iApply type_case_uniq; [solve_typing..|].
         constructor; last constructor; last constructor; left.
@@ -30,7 +32,7 @@ Section option_as_mut.
         iApply (type_jump [_]); solve_typing.
       + iApply (type_sum_assign [unit; &uniq{α}τ]%T); [solve_typing..|by apply write_own|].
         iApply (type_jump [_]); solve_typing.
-    - simpl. iIntros (k r). inv_vec r=>r. simpl_subst.
+    - iIntros "/= !#". iIntros (k r). inv_vec r=>r. simpl_subst.
       iApply type_delete; [solve_typing..|].
       iApply (type_jump [_]); solve_typing.
   Qed.
