theories/typing/examples/rebor.v
@@ -20,7 +20,8 @@ Section rebor.
     typed_instruction_ty [] [] [] rebor
         (fn([]; Π[int; int], Π[int; int]) → int).
   Proof.
-    iApply type_fn; [solve_typing..|]. simpl. iIntros ([] ret p). inv_vec p=>t1 t2. simpl_subst.
+    iApply type_fn; [solve_typing..|]. iIntros "/= !#". iIntros ([] ret p).
+       inv_vec p=>t1 t2. simpl_subst.
     iApply (type_newlft []). iIntros (α).
     iApply (type_letalloc_1 (&uniq{α}Π[int; int])); [solve_typing..|]. iIntros (x). simpl_subst.
     iApply type_deref; [solve_typing|apply read_own_move|done|]. iIntros (x'). simpl_subst.
