theories/typing/examples/unbox.v
@@ -15,7 +15,8 @@ Section unbox.
     typed_instruction_ty [] [] [] unbox
         (fn(∀ α, [☀α]; &uniq{α}box (Π[int; int])) → &uniq{α} int).
   Proof.
-    iApply type_fn; [solve_typing..|]. simpl. iIntros (α ret b). inv_vec b=>b. simpl_subst.
+    iApply type_fn; [solve_typing..|]. iIntros "/= !#". iIntros (α ret b).
+      inv_vec b=>b. simpl_subst.
     iApply type_deref; [solve_typing..|by apply read_own_move|done|].
     iIntros (b'); simpl_subst.
     iApply type_deref_uniq_own; [solve_typing..|]. iIntros (bx); simpl_subst.
